src/BetaEquiv.lean
@@ -10,15 +10,66 @@ open Term
 universe u
 variable {Var : Type u} [HasFresh Var] [DecidableEq Var]
 
+
+
+-- /-- A single β-reduction step. -/
+-- -- @[scoped grind]
+-- inductive Beta₂ : Term Var → Term Var → Prop
+-- /-- Reduce an application to a lambda term. -/
+-- | beta {M N : Term Var}: Beta₂ (app (abs M) N) (M ^ N)
+
+-- /-- Full β-reduction. -/
+-- @[reduction_sys "β₂"]
+-- abbrev FullBeta₂ : Term Var → Term Var → Prop := Xi Beta₂
+
+
+-- def Term.BetaEquiv₂ : Term Var → Term Var → Prop :=
+--   Relation.EqvGen FullBeta₂
+
+-- instance instEquivBetaEquiv : Equivalence (@BetaEquiv₂ Var) :=
+--   Relation.EqvGen.is_equivalence FullBeta₂
+
+-- lemma Beta_of_Beta₂ (M N X : Term Var) (hM : M.abs.LC) (hN : N.LC) (h : FullBeta₂ (M.abs.app N) X) : FullBeta (M.abs.app N) X := by
+--   -- apply Xi.base
+--   -- exact Xi.base (Beta.beta hM hN) M N
+--   -- constructor
+--   induction M
+
+  -- (abs M).app N ->β M
+
+  -- cases h with
+  -- | base h =>
+  --     constructor
+  --     cases h
+  --     constructor <;> assumption
+  -- | appL
+  -- · constructor
+  -- constructor <;> assumption
+
+
 notation3 t:39 " →βᶠ " t':39 => t ⭢βᶠ t'
 
 def Term.BetaEquiv : Term Var → Term Var → Prop :=
   Relation.EqvGen FullBeta
 
-instance : Equivalence (@BetaEquiv Var) :=
+instance instEquivBetaEquiv : Equivalence (@BetaEquiv Var) :=
   Relation.EqvGen.is_equivalence FullBeta
 
+instance : Setoid (Term Var) :=
+  {r := BetaEquiv
+   iseqv := instEquivBetaEquiv}
+
 notation M " ≡β " N => BetaEquiv M N
+
+@[symm]
+lemma BetaEquiv_symm {Var : Type u} {M N : Term Var} (h : M ≡β N) : N ≡β M := by
+  apply Relation.EqvGen.symm
+  exact h
+
+@[refl]
+lemma BetaEquiv_refl {Var : Type u} {M : Term Var} : M ≡β M := by
+  apply Relation.EqvGen.refl
+
 
 def idTerm := Term.abs $ @Term.bvar ℕ 0
 def betaRedex := Term.app (Term.abs $ @Term.bvar ℕ 0) (Term.abs $ @Term.bvar ℕ 0)
