src/LambdaTerms.lean
@@ -12,6 +12,6 @@ variable {Var : Type u}
 
 def K     : Term Var := abs (abs $ bvar 1) -- λxy.x
 def Kstar : Term Var := abs (abs $ bvar 0) -- λxy.y
-def id    : Term Var := abs (bvar 0)       -- λx.x
+def I     : Term Var := abs (bvar 0)       -- λx.x
 
 end LambdaTerms
