src/LambdaTheory/InconsistentTheories.lean
@@ -1,0 +1,332 @@
+import src.LambdaTheory.Basic
+import src.LambdaTerms
+import src.BetaEquiv
+import Cslib.Languages.LambdaCalculus.LocallyNameless.Untyped.FullBeta
+import Cslib.Languages.LambdaCalculus.LocallyNameless.Untyped.LcAt
+import Lean
+
+
+open Cslib
+open LambdaCalculus.LocallyNameless.Untyped
+open Term
+
+open LambdaTerms
+open LambdaTheory
+
+universe u
+variable {Var : Type u} [HasFresh Var] [DecidableEq Var]
+
+
+-- This file contains some examples of inconsistent theories
+
+section KeqKstar
+
+inductive ThKeqKstar : Term Var → Term Var → Prop
+| beta (M N) : FullBeta M N → ThKeqKstar M N
+| app (M N P Q) : ThKeqKstar M N → ThKeqKstar P Q → ThKeqKstar (Term.app M P) (Term.app N Q)
+-- | xi (M N) : LambdaRelated M N → Term.abs
+| refl (M) : ThKeqKstar M M
+| trans (M N P) : ThKeqKstar M N → ThKeqKstar N P → ThKeqKstar M P
+| sym (M N): ThKeqKstar M N → ThKeqKstar N M
+| new : ThKeqKstar K Kstar
+
+instance instKeqKstar : @LambdaTheory Var ThKeqKstar :=
+    ⟨ThKeqKstar.beta, ThKeqKstar.app, ThKeqKstar.refl, ThKeqKstar.trans, ThKeqKstar.sym⟩
+
+lemma ThKeqKstar_of_ThLambdaBeta {M N : Term Var} (h : ThLambdaBeta M N) : ThKeqKstar M N := by
+  induction h with
+  | beta _ _ h => apply ThKeqKstar.beta; assumption
+  | refl P => apply ThKeqKstar.refl
+  | sym M N h ih => apply ThKeqKstar.sym; assumption
+  | trans M N P _ _ hMN hNP =>
+    apply ThKeqKstar.trans M N P
+    · assumption
+    · assumption
+  | app M N P Q hMN hPQ _ _ =>
+    apply ThKeqKstar.app M N P Q
+    · assumption
+    · assumption
+
+lemma ThKeqKstar_of_BetaEquiv {M N : Term Var} (h : M ≡β N) : ThKeqKstar M N :=
+  ThKeqKstar_of_ThLambdaBeta (ThLambdaBeta_of_BetaEquiv h)
+
+lemma Kstar_LC {Var : Type u} : (@Kstar Var).LC := by
+  unfold Kstar
+  apply LC.abs
+  intro x _
+  apply LC.abs
+  intro y _
+  simp
+  apply LC.fvar
+  · exact Finset.empty
+  exact Finset.empty
+
+lemma reduceKstar {Var : Type u} (M : Term Var) (hM : M.LC) : (@app Var Kstar M) →βᶠ (abs $ bvar 0) := by
+  unfold Kstar
+
+  constructor
+  constructor
+  · apply LC.abs
+    intro x _
+    apply LC.abs
+    intro y _
+    simp
+    apply LC.fvar
+    · exact Finset.empty
+    · exact Finset.empty
+  · exact hM
+
+lemma reduceKstar2 {Var : Type u} (M N : Term Var) (hM : M.LC) (hN : N.LC) : (@app Var (@app Var Kstar M) N) ↠βᶠ N := by
+  -- unfold Kstar
+  apply Relation.ReflTransGen.tail (b := app (abs $ bvar 0) N)
+  apply Relation.ReflTransGen.single
+  apply Xi.appR
+  · assumption
+  · apply reduceKstar
+    · assumption
+  · constructor
+    constructor
+    apply LC.abs
+    grind
+    exact Finset.empty
+    assumption
+
+lemma K_LC {Var : Type u} : (@K Var).LC := by
+  unfold K
+  apply LC.abs
+  intro x _
+  apply LC.abs
+  intro y _
+  apply LC.fvar
+  · exact Finset.empty
+  exact Finset.empty
+
+
+lemma KstarMN_eq_N (M N : Term Var) (hM : M.LC) (hN : N.LC) : app (app Kstar M) N ≡β N := by
+  apply betaEquiv_of_multiBeta
+  · constructor
+    swap; assumption
+    constructor
+    swap; assumption
+    exact Kstar_LC
+  · assumption
+  · apply reduceKstar2
+    · assumption
+    · assumption
+
+lemma helper₃ {Var : Type u} (M O : Term Var) (hM : M.LC) (hO : O.LC) : (M.app O).LC := by
+  grind
+
+@[simp, grind .]
+lemma absLC_of_LC {M : Term Var} (h : M.LC): (abs M).LC := by
+    apply LC.abs
+    grind
+    exact Finset.empty
+
+@[simp, grind =]
+lemma openRec_abs_eq_abs_of_LC (M N : Term Var) (hM : M.LC) : (M.abs ^ N = M.abs) := by
+  induction M with
+  | bvar n => cases hM
+  | fvar x => cases hM with | fvar =>  unfold open'; simp_rw [openRec_abs, openRec_fvar]
+  | app M O ih₁ ih₂ =>
+    cases hM with | app hM hO =>
+      specialize ih₁ hM
+      specialize ih₂ hO
+      unfold open' at *
+      rw [openRec_abs] at ih₁
+      rw [openRec_abs] at ih₂
+      rw [openRec_abs, openRec_app]
+      simp
+      constructor
+      · simp only [zero_add, abs.injEq] at ih₁
+        exact ih₁
+      · simp only [zero_add, abs.injEq] at ih₂
+        exact ih₂
+  | abs M ih => grind only [= open'.eq_1, =_ open_lc, absLC_of_LC]
+
+@[simp, grind =]
+lemma test (M N : Term Var) (hM : M.LC) : M ^ N = M := by
+  grind
+
+-- -- (λx.M)
+lemma helper (M N : Term Var) (hM : M.LC) (hN : N.LC): app (abs M) N ↠βᶠ M:= by
+  induction M with
+  | abs O ih =>
+    apply Relation.ReflTransGen.single
+    apply Xi.base
+    have : (O.abs) = (O.abs) ^ N := by grind
+    nth_rw 2 [this]
+    apply Beta.beta
+    · grind
+    · assumption
+  | bvar n =>
+    apply Relation.ReflTransGen.single
+    apply Xi.base
+    have : bvar n = bvar n ^ N := by
+      grind
+    nth_rw 2 [this]
+    constructor
+    · grind
+    · assumption
+  | fvar x =>
+    apply Relation.ReflTransGen.single
+    apply Xi.base
+    have : fvar x = fvar x ^ N := by grind
+    nth_rw 2 [this]
+    constructor <;> try assumption
+    grind
+  | app M O ih₁ ih₂ =>
+    apply Relation.ReflTransGen.single
+    apply Xi.base
+    have : (M.app O) = (M.app O) ^ N := by grind
+    nth_rw 2 [this]
+    constructor <;> try assumption
+    grind
+
+  -- apply Relation.ReflTransGen.tail (b := M ^ N)
+  -- constructor
+
+
+lemma reduceK {Var : Type u} (M N : Term Var) (hM : M.LC) (hN : N.LC) : (app (app K M) N) ↠βᶠ M := by
+  unfold K
+  apply Relation.ReflTransGen.tail (b := app (abs M) N)
+  · apply Relation.ReflTransGen.single
+    apply Xi.appR
+    · exact hN
+    · constructor
+      constructor
+      apply LC.abs
+      · intro x _
+        apply LC.abs
+        intro y _
+        simp
+        apply LC.fvar
+        exact Finset.empty
+      · exact Finset.empty
+      · exact hM
+  · sorry
+
+
+
+
+instance : CoeFun (Term Var) (fun _ => Term Var → Term Var) where
+  coe M N := Term.app M N
+
+@[simp]
+lemma K_MN_eq_M (M N : Term Var) (hM : M.LC) (hN : N.LC) : app (app K M) N ≡β M := by
+  apply betaEquiv_of_multiBeta
+  · apply LC.app
+    · apply LC.app
+      · exact K_LC
+      · assumption
+    · assumption
+  · assumption
+  · apply reduceK
+    · assumption
+    · assumption
+
+local notation:50 M " =K= " N => ThKeqKstar M N
+
+-- We prove that adding K = Kstar results in an inconsistent λ-theory
+lemma K_eq_Kstart_inconsistent {Var : Type u} [instDec : DecidableEq Var] [instFresh : HasFresh Var] : @inconsistent Var ThKeqKstar instKeqKstar := by
+  intro M N hM hN
+
+  have h₁: M =K= K M N := by
+    simp
+    apply ThKeqKstar_of_BetaEquiv
+    apply BetaEquiv_symm
+    apply K_MN_eq_M
+    assumption
+    assumption
+
+  have h₂: K M N =K= Kstar M N := by
+    simp
+    apply app_left₂
+    apply ThKeqKstar.new
+
+  have h₃: Kstar M N =K= N := by
+    apply ThKeqKstar_of_BetaEquiv
+    apply KstarMN_eq_N
+    assumption
+    assumption
+
+  calc M =K= K M N := h₁
+       _ =K= Kstar M N := h₂
+       _ =K= N := h₃
+
+end KeqKstar
+
+section KeqI
+
+open Lean Elab Command
+
+syntax (name := deriveLambdaTheoryInstance)
+"mk_lambda_theory " ident : command
+
+@[command_elab deriveLambdaTheoryInstance]
+def elabDeriveLambdaTheoryInstance : CommandElab
+| `(mk_lambda_theory $thName:ident) => do
+  -- let thStr := thName.getId.toString
+
+  -- let instName := mkIdent <| Name.mkSimple s!"inst{thStr}"
+
+  let beta  := mkIdent <| thName.getId ++ `beta
+  let app   := mkIdent <| thName.getId ++ `app
+  let refl  := mkIdent <| thName.getId ++ `refl
+  let trans := mkIdent <| thName.getId ++ `trans
+  let sym   := mkIdent <| thName.getId ++ `sym
+
+  elabCommand <|
+    ← `(instance : @LambdaTheory Var $thName :=
+          ⟨$beta, $app, $refl, $trans, $sym⟩)
+| _ => throwUnsupportedSyntax
+
+-- @[LambdaTheory]
+inductive ThKeqI : Term Var → Term Var → Prop
+| beta (M N) : FullBeta M N → ThKeqI M N
+| app (M N P Q) : ThKeqI M N → ThKeqI P Q → ThKeqI (Term.app M P) (Term.app N Q)
+-- | xi (M N) : LambdaRelated M N → Term.abs
+| refl (M) : ThKeqI M M
+| trans (M N P) : ThKeqI M N → ThKeqI N P → ThKeqI M P
+| sym (M N): ThKeqI M N → ThKeqI N M
+| new : ThKeqI K I
+
+mk_lambda_theory ThKeqI
+
+-- instance instKeqI : @LambdaTheory Var ThKeqI :=
+--     ⟨ThKeqI.beta, ThKeqI.app, ThKeqI.refl, ThKeqI.trans, ThKeqI.sym⟩
+
+lemma ThKeqI_of_ThLambdaBeta {M N : Term Var} (h : ThLambdaBeta M N) : ThKeqI M N := by
+  induction h with
+  | beta _ _ h => apply ThKeqI.beta; assumption
+  | refl P => apply ThKeqI.refl
+  | sym M N h ih => apply ThKeqI.sym; assumption
+  | trans M N P _ _ hMN hNP =>
+    apply ThKeqI.trans M N P
+    · assumption
+    · assumption
+  | app M N P Q hMN hPQ _ _ =>
+    apply ThKeqI.app M N P Q
+    · assumption
+    · assumption
+
+lemma ThKeqI_of_BetaEquiv {M N : Term Var} (h : M ≡β N) : ThKeqI M N :=
+  ThKeqI_of_ThLambdaBeta (ThLambdaBeta_of_BetaEquiv h)
+
+local notation:50 M " =K= " N => ThKeqI M N
+
+-- M = K M N = I M N = K I I M N = I K I M N = K I M N = I N = N
+theorem KeqI_inconsistent : inconsistent (Var := Var) ThKeqI := by
+  intro M N hM hN
+
+  -- Th ⊨ M = N
+  -- TODO
+  calc M =K= K M N := by simp; sorry
+    _ =K= I M N := by simp; sorry
+    _ =K= K I I M N := by simp; sorry
+    _ =K= I K I M N := by simp; sorry
+    _ =K= K I M N := by simp; sorry
+    _ =K= I N := by simp; sorry
+    _ =K= N := by simp; sorry
+
+end KeqI
