src/LambdaTheory/LambdaBetaEta.lean
@@ -1,0 +1,32 @@
+import src.LambdaTheory.Basic
+import src.BetaEquiv
+import Cslib.Languages.LambdaCalculus.LocallyNameless.Untyped.FullBeta
+import Cslib.Languages.LambdaCalculus.LocallyNameless.Untyped.FullEta
+
+open Cslib
+open LambdaCalculus.LocallyNameless.Untyped
+open Term
+
+universe u
+variable {Var : Type u}
+
+
+open LambdaTheory
+
+section LambdaBetaEta
+
+inductive ThLambdaBetaEta : Term Var → Term Var → Prop
+| beta (M N) : FullBeta M N → ThLambdaBetaEta M N
+| app (M N P Q) : ThLambdaBetaEta M N → ThLambdaBetaEta P Q → ThLambdaBetaEta (app M P) (app N Q)
+-- | xi (M N) : LambdaRelated M N → Term.abs
+| refl (M) : ThLambdaBetaEta M M
+| trans (M N P) : ThLambdaBetaEta M N → ThLambdaBetaEta N P → ThLambdaBetaEta M P
+| sym (M N): ThLambdaBetaEta M N → ThLambdaBetaEta N M
+-- | eta (M) : LambdaBetaEta (abs (app M (bvar 0))) M -- TODO: Should be outer most
+
+#check FullEta
+
+instance : @LambdaTheory Var (ThLambdaBetaEta) :=
+  ⟨ThLambdaBetaEta.beta, ThLambdaBetaEta.app, ThLambdaBetaEta.refl, ThLambdaBetaEta.trans, ThLambdaBetaEta.sym⟩
+
+end LambdaBetaEta
